ifc-machine/pico/tmu/cmach/Concrete.v
@@ -35,26 +35,26 @@ Record CS  := CState {
   priv : bool
 }.
 
-(* Self contained code: [runsToEnd' pc1 pc2 cs1 cs2] starts at pc2
+(* Self contained code: [runsToEnd pc1 pc2 cs1 cs2] starts at pc2
 [pc1] and runs until pc [pc2]. *)
-Inductive runsToEnd' (Rstep: CS -> CS -> Prop) : Z -> Z -> CS -> CS -> Prop :=
-| runsToEndDone' : forall n cs,
+Inductive runsToEnd (Rstep: CS -> CS -> Prop) : Z -> Z -> CS -> CS -> Prop :=
+| runsToEndDone : forall n cs,
   fst (pc cs) = n -> 
-  runsToEnd' Rstep n n cs cs
+  runsToEnd Rstep n n cs cs
   (* NC: do we need to worry about [n <= n' <= n'']? *)
-| runsToEndStep': forall n n' n'' cs cs' cs'',
+| runsToEndStep: forall n n' n'' cs cs' cs'',
   fst (pc cs) = n ->
   Rstep cs cs' ->
   fst (pc cs') = n' ->
   n < n' ->
-  runsToEnd' Rstep n' n'' cs' cs'' -> 
-  runsToEnd' Rstep n  n'' cs  cs''.
+  runsToEnd Rstep n' n'' cs' cs'' -> 
+  runsToEnd Rstep n  n'' cs  cs''.
 
-Lemma runsToEnd'_compose : forall step pc0 pc1 s0 s1,
-  runsToEnd' step pc0 pc1 s0 s1 ->
+Lemma runsToEnd_compose : forall step pc0 pc1 s0 s1,
+  runsToEnd step pc0 pc1 s0 s1 ->
   forall pc2 s2,
-  runsToEnd' step pc1 pc2 s1 s2 ->
-  runsToEnd' step pc0 pc2 s0 s2.
+  runsToEnd step pc1 pc2 s1 s2 ->
+  runsToEnd step pc0 pc2 s0 s2.
 Proof.
   induction 1; intros; eauto.
   econstructor; eauto.
@@ -64,11 +64,11 @@ Qed.
   need to be more general than that, though  *)
 Inductive runsToEscape (Rstep : (CS -> CS -> Prop)) : Z -> Z -> CS -> CS -> Prop :=
 | rte_success: forall pc_start pc_end cs cs' cs'',
-               forall (TMU: runsToEnd' Rstep pc_start pc_end cs cs')
+               forall (TMU: runsToEnd Rstep pc_start pc_end cs cs')
                       (SUCC: Rstep cs' cs''),
                  runsToEscape Rstep pc_start pc_end cs cs''
 | rte_fail: forall pc_start pc_end cs cs',
-            forall (TMU: runsToEnd' Rstep pc_start pc_end cs cs')
+            forall (TMU: runsToEnd Rstep pc_start pc_end cs cs')
                    (FAIL: forall cs'', ~ Rstep cs' cs''),
               runsToEscape Rstep pc_start pc_end cs cs'
 | rte_upriv:forall pc_start pc_end cs,
